wip: working of OM state WF predicate

fairness/lawyer/obligations/obligations_model.v
@@ -183,200 +183,36 @@ Section Model.
     (exists s π δ δ', creates_ep ps1 θ ps2 s π δ δ') \/
     (exists s π δ, expects_ep ps1 θ ps2 s π δ).
 
+  Definition loc_step_of θ := fun ps1 ps2 => loc_step ps1 θ ps2. 
+  Definition fork_step_of θ := fun ps1 ps2 => exists τ' R, forks_locale ps1 θ ps2 τ' R. 
+
   Require Import Relation_Operators.
 
   Notation " x ;;; y " := (rel_compose x y) (at level 20).
 
   Definition progress_step ps1 (θ: Locale) ps2 :=
     exists n, n <= LIM_STEPS /\
-           (relations.nsteps (fun p1 p2 => loc_step p1 θ p2) n
+           (relations.nsteps (loc_step_of θ) n
              ;;;
             (fun p1 p2 => exists π δ, burns_cp p1 θ p2 π δ)
            )
             ps1 ps2.
 
+  Definition progress_step_of τ := fun δ1 δ2 => progress_step δ1 τ δ2.
+
   Definition om_trans ps1 (θ: Locale) ps2 :=
     exists ps',
       progress_step ps1 θ ps' /\
-      (clos_refl _ (fun p1 p2 => exists τ' R, forks_locale p1 θ p2 τ' R)) ps' ps2. 
+      (clos_refl _ (fork_step_of θ)) ps' ps2. 
                   
+  Definition om_trans_of τ := fun δ1 δ2 => om_trans δ1 τ δ2.
+
   Definition ObligationsModel: Model :=
     {| mtrans := om_trans |}. 
 
+  Definition phases_incompat π1 π2 := ¬ phase_le π1 π2 /\ ¬ phase_le π2 π1.
 
-    
-  (* Lemma burns_cp_th_obls_pres c τ δ1 δ2 d *)
-  (*   (BURN: burns_cp OP δ1 τ δ2 d) *)
-  (*   (TH_OWN: threads_own_obls c δ1): *)
-  (*   threads_own_obls c δ2. *)
-  (* Proof. *)
-  (*   inversion BURN; subst. *)
-  (*   by destruct δ1. *)
-  (* Qed. *)
-
-  (* (* TODO: rename *) *)
-  (* Lemma too_too' (c: cfg Λ) (δ: mstate OM) (θ: Phase) *)
-  (*   (IN: θ ∈ dom $ ps_obls OP δ) *)
-  (*   (TOO: thread_ *)
-
-  (* TODO: can be proved simpler if we could unfold ndot *)
-  Lemma ns_ndot_disj (ns: namespace) (i: nat):
-    ns ≠ ns .@ i.
-  Proof.
-    intros EQ.
-    pose proof (coPpick_elem_of (↑ ns .@ (i + 1)) (nclose_infinite _)) as IN.
-    pose proof IN as IN'. rewrite {2}EQ in IN'.
-    apply nclose_subseteq in IN'.
-    edestruct @ndot_ne_disjoint; [| apply IN | apply IN'].
-    lia.
-  Qed. 
-
-  (* TODO: can be proved simpler if we could unfold ndot *)
-  Lemma ns_ndot_diff_disj (ns: namespace) (i j: nat)
-    (NEQ: i ≠ j):
-    ns .@ i ≠ ns .@ j.
-  Proof.
-    intros EQ.
-    pose proof (coPpick_elem_of (↑ ns .@ i) (nclose_infinite _)) as IN1.
-    pose proof (coPpick_elem_of (↑ ns .@ j) (nclose_infinite _)) as IN2.
-    rewrite -{1}EQ in IN2. 
-    edestruct @ndot_ne_disjoint; [| apply IN1 | apply IN2].
-    done. 
-  Qed. 
-
-  (* Definition obls_corr (δ: mstate OM) (R: gset Phase) (θ: Phase) (b: bool) := *)
-  (*   θ ∉ R /\  *)
-  (*   if b  *)
-  (*   then dom (ps_obls OP δ) = (R ∖ {[ fork_left θ; fork_right θ ]} ∪ {[ θ ]}) /\ {[ fork_left θ; fork_right θ ]} ⊆ R *)
-  (*   else dom (ps_obls OP δ) = R.  *)
-
-  Definition obls_eq δ1 R := dom $ ps_obls δ1 = R.
-      
-  Lemma loc_step_obls_pres δ1 δ2 R θ
-    (LSTEP: loc_step δ1 θ δ2)
-    (OBLS_CORR: obls_eq δ1 R)
-    (* (DOMτ: is_Some (from_locale c.1 τ)): *)
-    :
-    obls_eq δ2 R.
-  Proof using.
-    (* clear H H0 H1.  *)
-    clear -LSTEP OBLS_CORR. 
-    add_case (dom $ ps_obls δ2 = dom $ ps_obls δ1) SAME.
-    { intros EQ. red. by rewrite EQ. }
-    
-    red in LSTEP. destruct LSTEP as [T|[T|[T|[T|[T|T]]]]].
-    - destruct T as (?&?&T). inversion T; subst.
-      apply SAME. by destruct δ1. 
-    - destruct T as (?&?&?&?&T). inversion T; subst. 
-      apply SAME. by destruct δ1. 
-    - destruct T as (?&T). inversion T; subst.
-      apply SAME. destruct δ1. simpl in *.
-      subst new_obls0. rewrite dom_insert_L. simpl. set_solver. 
-    - destruct T as (?&T). inversion T; subst.
-      apply SAME. destruct δ1. simpl in *.  
-      subst new_obls0. simpl.
-      rewrite dom_insert_L. 
-                                            set_solver. 
-    - destruct T as (?&?&?&?&T). inversion T; subst.
-      apply SAME. by destruct δ1. 
-    - destruct T as (?&?&?&T). inversion T; subst.
-      apply SAME. by destruct δ1.
-  Qed.     
-           
-  Lemma progress_step_obls_pres δ1 τ δ2 R
-    (STEP: progress_step δ1 τ δ2)
-    (TH_OWN: obls_eq δ1 R)
-    (* (DOMτ: is_Some (from_locale c.1 τ)) *)
-    :
-    obls_eq δ2 R.
-  Proof.
-    red in STEP. destruct STEP as (n&?&STEP).
-    eapply rel_compose_mono in STEP.
-    2: reflexivity.
-    1: apply rel_compose_nsteps_next in STEP.
-    2: { do 2 red. intros. by left. }
-    (* clear -(* DOMτ *) OM STEP TH_OWN. *)
-    generalize dependent δ2. induction n.
-    { simpl. intros ? ?%nsteps_once_inv. by eapply loc_step_obls_pres. }
-    intros ? (δ'&STEP1&STEP2)%rel_compose_nsteps_next.
-    apply IHn in STEP1. eapply loc_step_obls_pres; eauto.
-    lia. 
-  Qed.
-
-  Lemma obls_eq_init δ: obls_eq δ (dom $ ps_obls δ).
-  Proof. done. Qed. 
-    
-  Definition dom_phases_obls δ := dom $ ps_phases δ = dom $ ps_obls δ. 
-  Definition phases_eq δ1 R := ps_phases δ1 = R.
-
-  Lemma loc_step_phases_pres δ1 δ2 θ R
-    (LSTEP: loc_step δ1 θ δ2)
-    (PHASES_CORR: phases_eq δ1 R)
-    :
-    phases_eq δ2 R.
-  Proof using.
-    clear -LSTEP PHASES_CORR.
-    red in LSTEP. destruct LSTEP as [T|[T|[T|[T|[T|T]]]]].
-    - destruct T as (?&?&T). inversion T; subst.
-      by destruct δ1. 
-    - destruct T as (?&?&?&?&T). inversion T; subst. 
-      by destruct δ1. 
-    - destruct T as (?&T). inversion T; subst.
-      destruct δ1. simpl in *.
-      subst new_obls0. red. subst new_ps. simpl. set_solver. 
-    - destruct T as (?&T). inversion T; subst.
-      destruct δ1. simpl in *.  
-      subst new_obls0. simpl.
-      red. set_solver. 
-    - destruct T as (?&?&?&?&T). inversion T; subst.
-      by destruct δ1. 
-    - destruct T as (?&?&?&T). inversion T; subst.
-      by destruct δ1.
-  Qed. 
-
-  (* TODO: refactor *)
-  Lemma loc_step_nsteps_phases_pres δ1 δ2 θ R n
-    (LSTEPS: relations.nsteps (fun p1 p2 => loc_step p1 θ p2) n δ1 δ2)
-    (PHASES_CORR: phases_eq δ1 R)
-    :
-    phases_eq δ2 R.
-  Proof.
-    generalize dependent δ2. induction n.
-    { simpl. intros ? ->%nsteps_0. done. }
-    intros ? (δ'&STEP1&STEP2)%rel_compose_nsteps_next.
-    apply IHn in STEP1. eapply loc_step_phases_pres; eauto.
-  Qed. 
-
-  (* TODO: refactor *)
-  Lemma progress_step_phases_pres δ1 τ δ2 R
-    (STEP: progress_step δ1 τ δ2)
-    (DPO: phases_eq δ1 R)
-    (* (DOMτ: is_Some (from_locale c.1 τ)) *)
-    :
-    phases_eq δ2 R.
-  Proof.
-    red in STEP. destruct STEP as (n&?&STEP).
-    eapply rel_compose_mono in STEP.
-    2: reflexivity.
-    1: apply rel_compose_nsteps_next in STEP.
-    2: { do 2 red. intros. by left. }
-    eapply loc_step_nsteps_phases_pres; eauto.
-  Qed.
-
-  Lemma phases_eq_init δ: phases_eq δ (ps_phases δ).
-  Proof. done. Qed. 
-
-  (* TODO: refactor *)
-  Lemma progress_step_dpo_pres δ1 τ δ2
-    (STEP: progress_step δ1 τ δ2)
-    (DPO: dom_phases_obls δ1)
-    :
-    dom_phases_obls δ2.
-  Proof.
-    red. erewrite progress_step_obls_pres; [| eauto| apply obls_eq_init].
-    erewrite progress_step_phases_pres; [| eauto| apply phases_eq_init]. 
-    apply DPO. 
-  Qed.
+  Definition phase_lt := strict phase_le.  
 
   Global Instance phase_le_PreOrder: PreOrder phase_le.
   Proof.
@@ -385,8 +221,6 @@ Section Model.
     - set_solver.
     - red. set_solver.
   Qed.         
-  
-  Definition phase_lt := strict phase_le.
   
   Lemma phase_lt_fork π (d: nat):
     phase_lt π (π .@ d).
@@ -403,20 +237,6 @@ Section Model.
     lia.
   Qed. 
 
-  Definition phases_incompat π1 π2 := ¬ phase_le π1 π2 /\ ¬ phase_le π2 π1.
-
-  (* Definition phases_disjoint (π1 π2: Phase) := π1 ## π2.  *)
-  
-  (* Lemma phases_disjoint_incompat π1 π2: *)
-  (*   phases_disjoint π1 π2 -> phases_incompat π1 π2. *)
-  (* Proof using. *)
-  (*   rewrite /phases_disjoint /phases_incompat /phase_le. *)
-  (*   rewrite /disjoint /ndisjoint. intros DISJ. *)
-  (*   split; intros SUB.  *)
-  (*   - destruct (DISJ (coPpick (↑π2))); [apply SUB| ]; apply coPpick_elem_of, nclose_infinite.   *)
-  (*   - destruct (DISJ (coPpick (↑π1))); [| apply SUB]; apply coPpick_elem_of, nclose_infinite. *)
-  (* Qed.      *)
-  
   Global Instance phase_le_dec: forall x y, Decision (phase_le x y).
   Proof using. 
     intros. rewrite /phase_le. solve_decision. 
@@ -427,5 +247,244 @@ Section Model.
 
   Definition has_obls (τ: Locale) (s: mstate ObligationsModel) := default ∅ (ps_obls s !! τ) ≠ ∅. 
   Definition obls_trace_fair := fair_by has_obls eq.
+
+
+  (** Well-formedness of ProgressState *)
+  
+  Definition dom_phases_obls δ := dom $ ps_phases δ = dom $ ps_obls δ.
+
+  Definition obls_assigned δ :=
+    dom $ filter (fun '(s, (l, b)) => b = false) (ps_sigs δ) ⊆
+    flatten_gset $ map_img $ ps_obls δ.
+
+  Definition dom_phases_incompat δ :=
+    forall π1 π2, π1 ∈ (map_img $ ps_phases δ: gset Phase) -> 
+              π2 ∈ (map_img $ ps_phases δ: gset Phase) ->
+              π1 ≠ π2 -> phases_incompat π1 π2. 
+
+
+  Definition eps_phase_bound δ :=
+    ¬ (exists τ π ep, ps_phases δ !! τ = Some π /\
+                  ep ∈ ps_eps δ /\ phase_lt π ep.1.2).
+
+  Definition cps_phase_bound δ :=
+    ¬ (exists τ π cp, ps_phases δ !! τ = Some π /\
+                  cp ∈ ps_cps δ /\ phase_lt π cp.1).
+
+  Definition obls_disjoint δ :=
+    forall τ1 τ2, τ1 ≠ τ2 -> 
+             default ∅ (ps_obls δ !! τ1) ## default ∅ (ps_obls δ !! τ2).   
+
+  Record om_st_wf (δ: ProgressState) := {
+    om_wf_dpo: dom_phases_obls δ;
+    om_wf_asg: obls_assigned δ;
+    om_wf_ph_incompat: dom_phases_incompat δ;
+    om_wf_cps_ph_bound: cps_phase_bound δ;
+    om_wf_eps_ph_bound: eps_phase_bound δ;
+    om_wf_obls_disj: obls_disjoint δ;
+  }.
+
+  Definition preserved_by 
+    (R: ProgressState -> ProgressState -> Prop) (P: ProgressState -> Prop) :=
+    ∀ δ1 δ2, P δ1 -> R δ1 δ2 -> P δ2.
+  
+  Definition preserved_by_loc_step τ := preserved_by (loc_step_of τ).
+  Definition preserved_by_fork τ := preserved_by (fork_step_of τ).
+  Definition preserved_by_rep_loc_step τ :=
+    fun P => forall n, preserved_by (relations.nsteps (loc_step_of τ) n) P. 
+  Definition preserved_by_progress_step τ :=
+    preserved_by (progress_step_of τ). 
+  Definition preserved_by_om_trans τ :=
+    preserved_by (om_trans_of τ). 
+
+  Lemma pres_by_loc_step_implies_rep τ P
+    (PRES: preserved_by_loc_step τ P)
+    :
+    preserved_by_rep_loc_step τ P. 
+  Proof.
+    red. intros n. red. intros δ1.
+    induction n.
+    { simpl. intros ?? ->%nsteps_0. done. }
+    intros ?? (δ'&STEP1&STEP2)%rel_compose_nsteps_next.
+    apply IHn in STEP1; eauto.
+  Qed.
+
+  Lemma pres_by_loc_step_implies_progress τ P
+    (PPRES: preserved_by_loc_step τ P)
+    :
+    preserved_by_progress_step τ P. 
+  Proof using.
+    do 2 red. intros δ1 δ2 P1 STEP. 
+    red in STEP. destruct STEP as (n&?&STEP).
+    eapply rel_compose_mono in STEP.
+    2: reflexivity.
+    1: apply rel_compose_nsteps_next in STEP.
+    2: { do 2 red. intros. by left. }    
+    eapply pres_by_loc_step_implies_rep; eauto.
+  Qed.
+
+  Lemma pres_by_loc_fork_steps_implies_om_trans τ P
+    (PPRES: preserved_by_loc_step τ P)
+    (FPRES: preserved_by_fork τ P)
+    :
+    preserved_by_om_trans τ P. 
+  Proof using.
+    do 2 red. intros δ1 δ2 P1 STEP. 
+    red in STEP. destruct STEP as (?&PSTEP&FSTEP).
+    eapply pres_by_loc_step_implies_progress in PPRES.
+    do 2 red in PPRES. specialize_full PPRES; eauto.
+    inversion FSTEP; subst; try done.
+    eapply FPRES; eauto. 
+  Qed.
+
+  Ltac inv_loc_step STEP :=
+    destruct STEP as [T|[T|[T|[T|[T|T]]]]];
+    [destruct T as (?&?&T) |
+     destruct T as (?&?&?&?&T) |
+     destruct T as (?&T) |
+     destruct T as (?&T) |
+     destruct T as (?&?&?&?&T) |
+     destruct T as (?&?&?&T) ];
+    inversion T; subst. 
+
+  Lemma loc_step_dpo_pres τ: preserved_by_loc_step τ dom_phases_obls.
+  Proof using.
+    do 2 red. intros δ1 δ2 PHASES_CORR STEP.
+    inv_loc_step STEP; destruct δ1; try done; simpl in *. 
+    - subst new_obls0. red. subst new_ps. simpl. set_solver. 
+    - subst new_obls0. simpl. red. set_solver. 
+  Qed.
+
+  Lemma loc_step_asg_pres τ: preserved_by_loc_step τ obls_assigned.
+  Proof using.
+    do 2 red. intros δ1 δ2 ASG STEP.
+    inv_loc_step STEP; destruct δ1; try done; simpl in *. 
+    - subst new_ps. red. simpl.
+      subst new_sigs0 new_obls0. 
+      rewrite map_filter_insert. setoid_rewrite decide_True; [| done].
+      rewrite dom_insert_L.
+      rewrite map_img_insert_L.
+      rewrite flatten_gset_union flatten_gset_singleton.
+      rewrite (union_comm_L _ {[ _ ]}) -union_assoc_L.
+      apply union_mono; [done| ]. etrans; [apply ASG| ].
+      simpl.
+      apply elem_of_dom in DOM as [obls DOM].
+      erewrite <- (insert_id ps_obls0) at 1; eauto.
+      rewrite map_img_insert_L.
+      rewrite flatten_gset_union flatten_gset_singleton.
+      subst cur_loc_obls0. rewrite DOM. done.
+    - subst new_ps. red. simpl.
+      subst new_sigs0 new_obls0.
+      rewrite map_filter_insert. setoid_rewrite decide_False; [| done].
+      rewrite map_img_insert_L.
+      apply elem_of_dom in DOM as [obls DOM].
+      rewrite flatten_gset_union flatten_gset_singleton.
+      subst cur_loc_obls0. rewrite DOM. simpl.
+
+      apply elem_of_subseteq. intros s' DOM'. rewrite elem_of_union. 
+      rewrite elem_of_dom in DOM'. destruct DOM' as [[l' b'] DOM'].
+      apply map_filter_lookup_Some in DOM' as [DOM' ->].
+      apply lookup_delete_Some in DOM' as [NEQ DOM'].
+      forward eapply (@ASG s').
+      { simpl. apply elem_of_dom. eexists.
+        eapply map_filter_lookup_Some; eauto. split; done. }
+      simpl. intros ASG'.
+      apply flatten_gset_spec in ASG'. destruct ASG' as (obls'&ASG'&IN').
+      apply elem_of_map_img in ASG' as [τ' ASG'].
+      destruct (decide (τ' = τ)) as [-> | ]. 
+      { rewrite DOM in ASG'. inversion ASG'. subst. set_solver. }
+      right. apply flatten_gset_spec. eexists. split; eauto.
+      apply elem_of_map_img. eexists. eapply lookup_delete_Some; eauto.
+  Qed.
+
+  Lemma loc_step_dpi_pres τ: preserved_by_loc_step τ dom_phases_incompat.
+  Proof using.
+    do 2 red. intros δ1 δ2 DPI STEP.
+    inv_loc_step STEP; destruct δ1; try done; simpl in *.
+  Qed.
+
+  Definition phases_eq R δ1 := ps_phases δ1 = R.
+
+  Lemma loc_step_phases_pres τ R: preserved_by (loc_step_of τ) (phases_eq R).
+  Proof using. 
+    do 2 red. intros δ1 δ2 PH STEP.
+    inv_loc_step STEP; destruct δ1; try done; simpl in *.
+  Qed.
+
+  (* TODO: move *)
+  Lemma gmultiset_elem_of_weaken `{Countable K} (x y: gmultiset K) k:
+    k ∈ x ∖ y -> k ∈ x.
+  Proof using. multiset_solver. Qed. 
+
+  Lemma loc_step_epb_pres' τ: preserved_by_loc_step τ 
+                                (fun δ => eps_phase_bound δ /\ dom_phases_incompat δ). 
+  Proof using.
+    do 2 red. intros δ1 δ2 [EPB DPI] STEP.
+    split.
+    2: { eapply loc_step_dpi_pres; eauto. } 
+    pose proof (@loc_step_phases_pres _ _ _ _ ltac:(reflexivity) STEP) as PH.
+    add_case (ps_eps δ2 ⊆ ps_eps δ1) EPS_LE.
+    { intros LE. red. intros (τ' & π & ep & PH2 & IN & LT).
+      eapply elem_of_subseteq in IN; eauto.
+      rewrite PH in PH2. 
+      edestruct EPB; eauto. set_solver. }
+    inv_loc_step STEP; destruct δ1; try done; simpl in *.
+    red. intros (τ' & π & ep & PH2 & IN & LT).
+    subst new_ps new_eps0. simpl in IN.
+    apply elem_of_union in IN as [IN | IN].
+    { edestruct EPB; eauto. set_solver. }
+    apply elem_of_singleton in IN as ->. (* simpl in *. *)
+    simpl in *.
+
+    edestruct (DPI π π__max); simpl.
+    1, 2: by eapply elem_of_map_img; eauto.
+    all: set_solver. 
+  Qed. 
+
+  Lemma loc_step_cpb_pres' τ: preserved_by_loc_step τ
+                                (fun δ => cps_phase_bound δ /\ dom_phases_incompat δ). 
+  Proof using.
+    do 2 red. intros δ1 δ2 [CPB DPI] STEP.
+    split.
+    2: by eapply loc_step_dpi_pres; eauto. 
+    pose proof (@loc_step_phases_pres _ _ _ _ ltac:(reflexivity) STEP) as PH.
+    add_case (ps_cps δ2 ⊆ ps_cps δ1) CPS_LE.
+    { intros LE. red. intros (τ' & π & cp & PH2 & IN & LT).
+      eapply gmultiset_elem_of_subseteq in IN; eauto.
+      rewrite PH in PH2. 
+      edestruct CPB; eauto. set_solver. }
+    
+    inv_loc_step STEP; destruct δ1; try done; simpl in *.
+    - apply CPS_LE. multiset_solver.
+    - red. simpl. intros (τ' & π & cp & PH2 & IN & LT).
+      subst new_cps0. rewrite gmultiset_elem_of_disj_union in IN.
+      destruct IN as [IN | IN].
+      { apply gmultiset_elem_of_weaken in IN.
+        edestruct CPB; eauto. set_solver. }
+      apply gmultiset_elem_of_scalar_mul in IN as [? IN].
+      apply gmultiset_elem_of_singleton in IN as ->. simpl in *.
+      edestruct CPB; eauto. set_solver.
+    - apply CPS_LE. multiset_solver.
+    - red. simpl. intros (τ' & π & cp & PH2 & IN & LT).
+      subst new_cps0. rewrite gmultiset_elem_of_disj_union in IN.
+      destruct IN as [IN | IN].
+      { edestruct CPB; eauto. set_solver. }
+      apply gmultiset_elem_of_singleton in IN as ->. simpl in *.
+      edestruct (DPI π π__max); simpl.
+      1, 2: by eapply elem_of_map_img; eauto.
+      all: set_solver. 
+  Qed.
+
+  Lemma wf_preserved_by_loc_step τ: preserved_by (loc_step_of τ) om_st_wf.
+  Proof using.
+    red. intros ?? WF1 STEP. 
+    split.
+    - eapply loc_step_dpo_pres; eauto. apply WF1.
+    - eapply loc_step_asg_pres; eauto. apply WF1.  
+    - eapply loc_step_dpi_pres; eauto. apply WF1.
+    - eapply loc_step_cpb_pres'; eauto. split; apply WF1.
+    - eapply loc_step_epb_pres'; eauto. split; apply WF1.
+    - 
+
 
 End Model.
